ShifFVars

src/Sound/Context.dfy
@@ -1,15 +1,233 @@
 module Context {
   import opened Defs
 
+    function SeqDepthExpr(ss: seq<Expr>): Idx 
+    {
+      if ss == [] then 0 else max(ss[0].Depth(), SeqDepthExpr(ss[1..]))
+    }
+
+
+  function SeqMax(ss: seq<Idx>): Idx 
+    ensures forall i <- ss :: i <= SeqMax(ss)
+    ensures forall i: nat :: i < |ss| ==> ss[i] <= SeqMax(ss)
+  {
+    if ss == [] then 
+      0 
+    else
+      assert ss == [ss[0]] + (ss[1..]);
+      max(ss[0], SeqMax(ss[1..]))
+  }
+
   datatype Context = Context(
+    ctx: seq<Expr>,
+    incarnation: seq<nat>) 
+  {
+    ghost const Models : iset<State> := iset st: State | IsSatisfiedOn(st)
+
+    ghost const AdjustedModels : iset<State> := 
+      iset st: State | exists st' <- Models {:InAdjustedModelsLemma(st')} :: AdjustState(st') == st
+
+    lemma InAdjustedModelsLemma(st: State, st': State)
+      requires IsSatisfiedOn(st')
+      requires st == AdjustState(st')
+      ensures st in AdjustedModels
+    {
+
+    }
+
+    function Depth(): Idx 
+    {
+      max(SeqDepthExpr(ctx), SeqMax(incarnation))
+    }
+
+    function FreshIdx(): Idx
+      ensures forall i <- incarnation :: i < FreshIdx()
+    {
+      SeqMax(incarnation) + 1
+    }
+
+    
+
+    function AdjustState(s: State): State
+      requires forall i <- incarnation :: i < |s|
+    { 
+      // Q: how to get rid of `if`?
+      seq(|incarnation|, i => 
+        if 0 <= i < |incarnation| then
+          assert incarnation[i] in incarnation;
+          s[incarnation[i]]
+        else true)
+    }
+
+    function SubstituteIdx(e: Expr, i: Idx): Expr
+      requires e.IsDefinedOn(|incarnation| + i)
+      decreases e
+    {
+      match e
+      case BConst(bvalue) => e
+      case BVar(v) =>
+        if v >= i then  
+          BVar(incarnation[v - i] + i) 
+        else e
+      case And(e0, e1) => 
+        And(SubstituteIdx(e0, i), SubstituteIdx(e1, i))
+      case Or(e0, e1) => 
+        Or(SubstituteIdx(e0, i), SubstituteIdx(e1, i))
+      case Not(e) => 
+        Not(SubstituteIdx(e, i))
+      case Implies(e0, e1) => 
+        Implies(SubstituteIdx(e0, i), SubstituteIdx(e1, i))
+      case Forall(v, body) => 
+        Forall(v, SubstituteIdx(body, i + 1))
+    }
+
+    function Substitute(e: Expr): Expr
+      requires e.IsDefinedOn(|incarnation|)
+    {
+      SubstituteIdx(e, 0)
+    }
+
+    function MkEntailment(e: Expr): Expr
+      requires e.IsDefinedOn(|incarnation|)
+    {
+      Implies(Conj(ctx), Substitute(e))
+    }
+
+    function Add(e: Expr): Context
+      requires e.IsDefinedOn(|incarnation|)
+    {
+      this.(ctx := ctx + [Substitute(e)])
+    }
+
+    method AddEq(v: Idx, e: Expr) returns (ghost vNew: Idx, context: Context)
+      requires v < |incarnation|
+      requires e.IsDefinedOn(|incarnation|)
+      ensures |incarnation| == |context.incarnation|
+      ensures ctx + [Eq(BVar(vNew), Substitute(e))] == context.ctx
+      ensures incarnation[v := vNew] == context.incarnation
+      ensures forall i <- incarnation :: i < vNew 
+      ensures vNew == SeqMax(incarnation) + 1
+      ensures SeqMax(incarnation) + 1 == SeqMax(context.incarnation)
+    {
+      var v' := FreshIdx();
+      var ctx' := ctx + [Eq(BVar(v'), Substitute(e))];
+      // FVarsEqLemma(Var(v'), Substitute(e));
+      // FVarsConjUnionLemma(ctx, [Eq(Var(v'), Substitute(e))]);
+      var incarnation' := incarnation[v := v'];
+      context := Context(ctx', incarnation');
+      vNew := v';
+    }
+
+    method AddVar() returns (ghost vNew: Idx, context: Context)
+      ensures context.incarnation == [vNew] + incarnation
+      ensures context.ctx         == ctx
+
+      ensures forall i <- incarnation :: i < vNew 
+      ensures vNew == SeqMax(incarnation) + 1
+      ensures SeqMax(incarnation) + 1 == SeqMax(context.incarnation)
+    {
+      var v' := FreshIdx();
+      var incarnation' :=  [v'] + incarnation;
+      context := Context(ctx, incarnation');
+      vNew := v';
+    }
+
+    ghost predicate IsDefinedOn(d: Idx)
+    {
+      forall e <- ctx :: e.IsDefinedOn(d)
+    }
+
+    ghost predicate IsSatisfiedOn(s: State) 
+    {
+      && IsDefinedOn(|s|) 
+      && (|s| == SeqMax(incarnation) + 1)
+      && (forall i <- incarnation :: i < |s|)
+      && (forall e <- ctx :: s.Eval(e))
+    }
+
+    ghost predicate Entails(e: Expr) 
+    {
+      forall s: State ::  
+        e.IsDefinedOn(|s|) && IsSatisfiedOn(s) ==> s.Eval(e)
+    }
+
+    lemma SubstituteIdxIsDefinedOnLemma(e: Expr, i: Idx, d: Idx)
+      requires e.IsDefinedOn(|incarnation| + i)
+      requires forall ic <- incarnation :: ic + i < d
+      requires i <= d
+      ensures SubstituteIdx(e, i).IsDefinedOn(d)
+      decreases e
+    {
+      match e 
+      case BVar(v) => if v >= i { assert incarnation[v - i] in incarnation; }
+      case Forall(v, body) => SubstituteIdxIsDefinedOnLemma(body, i + 1, d + 1);
+      case _ =>
+    }
+
+    lemma SubstituteIsDefinedOnLemma(e: Expr, d: Idx)
+      requires e.IsDefinedOn(|incarnation|)
+      requires forall ic <- incarnation :: ic < d
+      ensures Substitute(e).IsDefinedOn(d)
+      decreases e
+    {
+      SubstituteIdxIsDefinedOnLemma(e, 0, d);
+    }
+
+    lemma ForallPush(s1: State, s2: State, e1: Expr, e2: Expr)
+      requires e1.IsDefinedOn(|s1| + 1)
+      requires e2.IsDefinedOn(|s2| + 1)
+      requires forall b: bool :: s1.Update(b).Eval(e1) == s2.Update(b).Eval(e2)
+      ensures (forall b: bool :: s1.Update(b).Eval(e1)) == (forall b: bool :: s2.Update(b).Eval(e2))
+    { }
+
+    lemma AdjustStateSubstituteIdxLemma(s: State, e: Expr, i: Idx)
+      requires e.IsDefinedOn(|incarnation| + i)
+      requires forall ic <- incarnation :: ic + i < |s|
+      requires i <= |s|
+      ensures (SubstituteIdxIsDefinedOnLemma(e, i, |s|);
+        (s[..i] + AdjustState(s[i..])).Eval(e)) == s.Eval(SubstituteIdx(e, i))
+      decreases e
+    {
+      match e 
+      case Forall(v, body) =>
+        SubstituteIdxIsDefinedOnLemma(e, i, |s|);
+        assert forall b: bool :: ((s[..i] + AdjustState(s[i..])).Update(b)).Eval(body) == (s.Update(b)).Eval(SubstituteIdx(body, i + 1)) by {
+          forall b: bool ensures ((s[..i] + AdjustState(s[i..])).Update(b)).Eval(body) == (s.Update(b)).Eval(SubstituteIdx(body, i + 1)) {
+            assert ([b] + s)[..i+1] == [b] + s[..i];
+            assert ([b] + s)[i+1..] == s[i..];
+            assert ((s[..i] + AdjustState(s[i..])).Update(b)) == (([b] + s)[..i+1] + AdjustState(([b] + s)[i+1..]));
+            AdjustStateSubstituteIdxLemma([b] + s, body, i + 1);
+          }
+        }
+        ForallPush(s[..i] + AdjustState(s[i..]), s, body, SubstituteIdx(body, i + 1));
+      case BVar(v) => if v >= i { assert incarnation[v - i] in incarnation; }
+      case _  => 
+    }
+
+    lemma AdjustStateSubstituteLemma(s: State, e: Expr)
+      requires e.IsDefinedOn(|incarnation|)
+      requires forall ic <- incarnation :: ic < |s|
+      ensures Substitute(e).IsDefinedOn(|s|)
+      ensures AdjustState(s).Eval(e) == s.Eval(Substitute(e))
+    {
+      SubstituteIsDefinedOnLemma(e, |s|);
+      AdjustStateSubstituteIdxLemma(s, e, 0);
+      assert [] + AdjustState(s) == AdjustState(s);
+    }
+
+  }
+}
+
+  /*datatype Context = Context(P
     ctx: seq<Expr>, 
-    incarnation: map<Variable, Variable>, 
+    incarnation: seq<Variable>,
     bVars: set<Variable>) 
   {
 
-    ghost const Models : iset<State> := iset st: State | IsSatisfiedOn(st)
+    /*ghost const Models : iset<State> := iset st: State | IsSatisfiedOn(st)
     // Q: is it correct way to set a trigger?
-    ghost const AdjustedModels : iset<State> := iset st: State | exists st' <- Models {:InAdjustedModelsLemma(st')} :: AdjustState(st') == st
+    ghost const AdjustedModels : iset<State> := 
+      iset st: State | exists st' <- Models {:InAdjustedModelsLemma(st')} :: AdjustState(st') == st
 
     lemma InAdjustedModelsLemma(st: State, st': State)
       requires IsSatisfiedOn(st')
@@ -204,8 +422,8 @@ module Context {
                   }
                 }
               }
-            ctx'.AdjustStateSubstituteLemma'(s.Update(v, b), body);
-          }
+              ctx'.AdjustStateSubstituteLemma'(s.Update(v, b), body);
+            }
         }
       case Var(v) =>
       case BConst(bvalue) =>
@@ -231,7 +449,7 @@ module Context {
       ensures (
         SubstituteIsDefinedOnLemma(e); 
         AdjustState(s).Eval(e) == s.Eval(Substitute(e)))
-    { AdjustStateSubstituteLemma'(s, e); }
+    { AdjustStateSubstituteLemma'(s, e); }*/
   }
 
-}
+}*/
