src/Sound/Defs.dfy
@@ -1,14 +1,21 @@
 module Defs { 
 
-  ghost function UpdateSet(v: Variable, post: iset<State>): iset<State> 
+  function Tail(ss: State): State {
+    if ss == [] then [] else ss[1..]
+  }
+
+  ghost function UpdateSet(post: iset<State>): iset<State> 
   {
-    iset st: State | st - {v} in post
+    iset st: State | Tail(st) in post 
   }
 
-  ghost function DeleteSet(v: Variable, post: iset<State>): iset<State> {
-    iset st: State | exists st' <- post :: st == st' - {v}
+  ghost function DeleteSet(post: iset<State>): iset<State> {
+    iset st: State | exists st' <- post :: st == Tail(st')
   }
 
+  function max(x: nat, y: nat): nat {
+    if x > y then x else y
+  }
 
   ghost const AllStates: iset<State> := iset st: State | true
 
@@ -30,28 +37,8 @@ module Defs {
       res
     }
   }
-
-  function ExceptUpdate(e: Except<State>, v: Variable, b: bool): Except<State> {
-    var r :- e;
-    Ok(r.Update(v, b))
-  }
-
-  function ExceptRemove(e: Except<State>, v: Variable): Except<State> {
-    var r :- e;
-    Ok(r - {v})
-  }
-
-  // import opened Values
-
-  // class Variable
-  // {
-  //   const name: string
-
-  //   constructor (name: string) {
-  //     this.name := name;
-  //   }
-  // }
   type Variable = string
+  type Idx = nat
 
   datatype Expr =
     | BConst(bvalue: bool)
@@ -59,78 +46,77 @@ module Defs {
     | Or(0: Expr, 1: Expr)
     | Not(e: Expr)
     | Implies(0: Expr, 1: Expr)
-    | Var(v: Variable)
+    | BVar(id: Idx)
     | Forall(v: Variable, body: Expr) 
   {
-    function FVars(): set<Variable> {
+    function Depth(): Idx {
       match this
-      case BConst(_) => {}
-      case And(e0, e1) => e0.FVars() + e1.FVars()
-      case Or(e0, e1) => e0.FVars() + e1.FVars()
-      case Not(e) => e.FVars()
-      case Implies(e0, e1) => e0.FVars() + e1.FVars()
-      case Forall(v, body) => body.FVars() - {v}
-      case Var(v) => {v}
+      case BConst(_) => 0
+      case And(e0, e1) => max(e0.Depth(), e1.Depth())
+      case Or(e0, e1) => max(e0.Depth(), e1.Depth())
+      case Not(e) => e.Depth()
+      case Implies(e0, e1) => max(e0.Depth(), e1.Depth())
+      case BVar(id) => id + 1
+      case Forall(v, body) => if body.Depth() == 0 then 0 else body.Depth() - 1
     }
 
-    function BVars(): set<Variable> {
-      match this
-      case BConst(_) => {}
-      case And(e0, e1) => e0.BVars() + e1.BVars()
-      case Or(e0, e1) => e0.BVars() + e1.BVars()
-      case Not(e) => e.BVars()
-      case Implies(e0, e1) => e0.BVars() + e1.BVars()
-      case Forall(v, body) => body.BVars() + {v}
-      case Var(v) => {}
+    predicate IsDefinedOn(d: Idx) {
+      Depth() <= d
     }
 
-    predicate IsDefinedOn(s: set<Variable>) {
-      FVars() <= s
-    }
 
-    predicate NoShadowing() {
-      match this
-      case BConst(_) => true
-      case Var(v) => true
-      case And(e0, e1) => e0.NoShadowing() && e1.NoShadowing()
-      case Or(e0, e1) => e0.NoShadowing() && e1.NoShadowing()
-      case Not(e) => e.NoShadowing()
-      case Implies(e0, e1) => e0.NoShadowing() && e1.NoShadowing()
-      case Forall(v, body) => v !in body.BVars() && body.NoShadowing()
-    }
-
-    predicate WellFormed() {
-      NoShadowing()
-    }
-    
-    lemma IsDefinedOnTransitivity(s1: set<Variable>, s2: set<Variable>)
-        requires s1 <= s2
-        ensures IsDefinedOn(s1) ==> IsDefinedOn(s2)
+    lemma IsDefinedOnTransitivity(d1: Idx, d2: Idx)
+        requires d1 <= d2
+        ensures IsDefinedOn(d1) ==> IsDefinedOn(d2)
     {  }
 
     ghost predicate Holds() {
-      forall s: State :: IsDefinedOn(s.Keys) ==> s.Eval(this)
+      forall s: State :: IsDefinedOn(|s|) ==> s.Eval(this)
     }
 
-    lemma IsDefinedOnFVarsLemma(s: State, v: Variable)
-      requires v !in FVars()
-      ensures IsDefinedOn(s.Keys + {v}) ==> IsDefinedOn(s.Keys)
-    {  }
+    // lemma IsDefinedOnFVarsLemma(s: State, v: Variable)
+    //   requires v !in FVars()
+    //   ensures IsDefinedOn(s.Keys + {v}) ==> IsDefinedOn(s.Keys)
+    // {  }
 
-    lemma EvalFVarsLemma(s1: State, s2: State) 
-      requires IsDefinedOn(s1.Keys)
-      requires IsDefinedOn(s2.Keys)
-      requires forall v: Variable :: v in FVars() ==> s1[v] == s2[v]
+    lemma EvalDepthLemma(s1: State, s2: State) 
+      requires IsDefinedOn(|s1|)
+      requires IsDefinedOn(|s2|)
+      requires forall i: Idx :: i < Depth() ==> s1[i] == s2[i]
       ensures s1.Eval(this) == s2.Eval(this)
 
     { 
       match this
       case Forall(v, body) => 
         forall x: bool { 
-          body.EvalFVarsLemma(s1.Update(v, x), s2.Update(v, x)); 
+          body.EvalDepthLemma(s1.Update(x), s2.Update(x)); 
         }
       case _ =>
     }
+
+    function ShiftFVars(i: Idx): Expr {
+      match this
+      case Forall(v, body) => Forall(v, body.ShiftFVars(i + 1))
+      case BVar(v) => if v >= i then BVar(v + 1) else BVar(v)
+      case And(e0, e1) => And(e0.ShiftFVars(i), e1.ShiftFVars(i))
+      case Or(e0, e1) => Or(e0.ShiftFVars(i), e1.ShiftFVars(i))
+      case Not(e) => Not(e.ShiftFVars(i))
+      case Implies(e0, e1) => Implies(e0.ShiftFVars(i), e1.ShiftFVars(i))
+      case _ => this
+    }
+
+    // lemma ShiftFVarsDepthLemma(i: Idx)
+    //   ensures ShiftFVars(i).Depth() == Depth() + i
+    // {
+    //   match this 
+    //   case Forall(v, body) => body.ShiftFVarsDepthLemma(i + 1);
+    //   case BVar(v) => 
+    //   if v >= i {
+
+    //   } else {
+    //   }
+    //   case _ =>
+    // }
       
   }
 
@@ -138,13 +124,13 @@ module Defs {
     And(Implies(e1, e2), Implies(e2, e1))
   }
 
-  lemma FVarsEqLemma(e1: Expr, e2: Expr)
-    ensures Eq(e1, e2).FVars() == e1.FVars() + e2.FVars()
+  lemma DepthEqLemma(e1: Expr, e2: Expr)
+    ensures Eq(e1, e2).Depth() == max(e1.Depth(), e2.Depth())
   {  }
 
   lemma EvalEqLemma(e1: Expr, e2: Expr, s: State)
-    requires e1.IsDefinedOn(s.Keys)
-    requires e2.IsDefinedOn(s.Keys)
+    requires e1.IsDefinedOn(|s|)
+    requires e2.IsDefinedOn(|s|)
     requires s.Eval(e1) == s.Eval(e2)
     ensures s.Eval(Eq(e1, e2))
   {  }
@@ -153,7 +139,7 @@ module Defs {
     | Check(e: Expr)
     | Assume(e: Expr)
     | Seq(ss: seq<Stmt>)
-    | Assign(lhs: Variable, rhs: Expr)
+    | Assign(lhs: Idx, rhs: Expr)
     | VarDecl(v: Variable, s: Stmt)
     // | Loop(inv: Expr, body: Stmt)
     // | While(guard: Expr, inv: Expr, body: Stmt)
@@ -169,48 +155,87 @@ module Defs {
       case VarDecl(_, s) => 1 + s.Size()
     }
 
-    function FVars(): set<Variable> {
+    function Depth(): Idx {
       match this
-      case Check(e) => e.FVars()
-      case Assume(e) => e.FVars()
-      case Seq(ss) => SeqFVars(ss)
-      case Assign(lhs, rhs) => {lhs} + rhs.FVars()
-      case VarDecl(v, s) => s.FVars() - {v}
-      case Choice(s0, s1) => s0.FVars() + s1.FVars()
+      case Check(e) => e.Depth()
+      case Assume(e) => e.Depth()
+      case Seq(ss) => SeqDepth(ss)
+      case Assign(id, rhs) => max(id + 1, rhs.Depth())
+      case VarDecl(_, s) => if s.Depth() == 0 then 0 else s.Depth() - 1
+      case Choice(s0, s1) => max(s0.Depth(), s1.Depth())
     }
 
-    function BVars(): set<Variable> {
+    function ShiftFVars(i: Idx): Stmt {
       match this
-      case Check(e) => e.BVars()
-      case Assume(e) => e.BVars()
-      case Seq(ss) => SeqBVars(ss)
-      case Assign(lhs, rhs) => rhs.BVars()
-      case VarDecl(v, s) => s.BVars() + {v}
-      case Choice(s0, s1) => s0.BVars() + s1.BVars()
+      case Check(e) => Check(e.ShiftFVars(i))
+      case Assume(e) => Assume(e.ShiftFVars(i))
+      case Seq(ss) => Seq(SeqShiftFVars(ss, i))
+      case Assign(id, rhs) =>
+        if id >= i then 
+          Assign(id + 1, rhs.ShiftFVars(i)) 
+        else Assign(id, rhs.ShiftFVars(i))
+      case VarDecl(v, s) => VarDecl(v, s.ShiftFVars(i + 1))
+      case Choice(s0, s1) => Choice(s0.ShiftFVars(i), s1.ShiftFVars(i))
     }
 
-    predicate NoShadowing() {
-      match this
-      case Check(e) => e.NoShadowing()
-      case Assume(e) => e.NoShadowing()
-      case Seq(ss) => SeqNoShadowing(ss, this)
-        // && SeqNoShadowingNested(ss)
-        // && (forall i, j :: 0 <= i < j < |ss| ==> ss[i].BVars() !* ss[j].BVars())
-      case Assign(lhs, rhs) => rhs.NoShadowing()
-      case VarDecl(v, s) => v !in s.BVars() && s.NoShadowing()
-      case Choice(s0, s1) => s0.NoShadowing() && s1.NoShadowing()
+    lemma ShiftFVarsSizeLemma(i: Idx)
+      ensures ShiftFVars(i).Size() == Size()
+    {
+      match this 
+      case Seq(ss) => SeqShiftFVarsSizeLemma(ss, i);
+      case _ =>
     }
 
-    predicate WellFormed() {
-      NoShadowing() && FVars() !! BVars()
-    }
+    // lemma ShiftFVarsDepthLemma(i: Idx)
+    //   ensures ShiftFVars(i).Depth() == Depth() + i
+    // {
+    //   match this 
+    //   case Seq(ss) => SeqShiftFVarsDepthLemma(ss, i);
+    //   case _ =>
+    // }
 
-    predicate IsDefinedOn(s: set<Variable>) {
-      FVars() <= s
+    // function FVars(): set<Variable> {
+    //   match this
+    //   case Check(e) => e.FVars()
+    //   case Assume(e) => e.FVars()
+    //   case Seq(ss) => SeqFVars(ss)
+    //   case Assign(lhs, rhs) => {lhs} + rhs.FVars()
+    //   case VarDecl(v, s) => s.FVars() - {v}
+    //   case Choice(s0, s1) => s0.FVars() + s1.FVars()
+    // }
+
+    // function BVars(): set<Variable> {
+    //   match this
+    //   case Check(e) => e.BVars()
+    //   case Assume(e) => e.BVars()
+    //   case Seq(ss) => SeqBVars(ss)
+    //   case Assign(lhs, rhs) => rhs.BVars()
+    //   case VarDecl(v, s) => s.BVars() + {v}
+    //   case Choice(s0, s1) => s0.BVars() + s1.BVars()
+    // }
+
+    // predicate NoShadowing() {
+    //   match this
+    //   case Check(e) => e.NoShadowing()
+    //   case Assume(e) => e.NoShadowing()
+    //   case Seq(ss) => SeqNoShadowing(ss, this)
+    //     // && SeqNoShadowingNested(ss)
+    //     // && (forall i, j :: 0 <= i < j < |ss| ==> ss[i].BVars() !* ss[j].BVars())
+    //   case Assign(lhs, rhs) => rhs.NoShadowing()
+    //   case VarDecl(v, s) => v !in s.BVars() && s.NoShadowing()
+    //   case Choice(s0, s1) => s0.NoShadowing() && s1.NoShadowing()
+    // }
+
+    // predicate WellFormed() {
+    //   NoShadowing() && FVars() !! BVars()
+    // }
+
+    predicate IsDefinedOn(d: Idx) {
+      Depth() <= d
     }
-    lemma IsDefinedOnTransitivity(s1: set<Variable>, s2: set<Variable>)
-      requires s1 <= s2
-      ensures IsDefinedOn(s1) ==> IsDefinedOn(s2)
+    lemma IsDefinedOnTransitivity(d1: Idx, d2: Idx)
+      requires d1 <= d2
+      ensures IsDefinedOn(d1) ==> IsDefinedOn(d2)
     {  }
 
     predicate Single() {
@@ -231,28 +256,54 @@ module Defs {
     ensures SeqSize(ss) == ss[0].Size() + SeqSize(ss[1..])
   {  }
 
-  function SeqFVars(ss: seq<Stmt>): set<Variable> 
-    decreases ss
-  {
-    if ss == [] then {} else ss[0].FVars() + SeqFVars(ss[1..])
+  function SeqDepth(ss: seq<Stmt>): nat {
+    if ss == [] then 0 else max(ss[0].Depth(), SeqDepth(ss[1..]))
   }
 
-  function SeqBVars(ss: seq<Stmt>): set<Variable> {
-    if ss == [] then {} else ss[0].BVars() + SeqBVars(ss[1..])
+  function SeqShiftFVars(ss: seq<Stmt>, i: Idx): seq<Stmt> {
+    if ss == [] then [] else [ss[0].ShiftFVars(i)] + SeqShiftFVars(ss[1..], i)
   }
+
+  lemma SeqShiftFVarsSizeLemma(ss: seq<Stmt>, i: Idx)
+    ensures SeqSize(SeqShiftFVars(ss, i)) == SeqSize(ss)
+  {
+    if ss != [] {
+      assert ss == [ss[0]] + (ss[1..]);
+      ss[0].ShiftFVarsSizeLemma(i);
+    }
+  }
+
+  // lemma SeqShiftFVarsDepthLemma(ss: seq<Stmt>, i: Idx)
+  //   ensures SeqDepth(SeqShiftFVars(ss, i)) == SeqDepth(ss) + i
+  // {
+  //   if ss != [] {
+  //     assert ss == [ss[0]] + (ss[1..]);
+  //     ss[0].ShiftFVarsDepthLemma(i);
+  //   }
+  // }
+
+  // function SeqFVars(ss: seq<Stmt>): set<Variable> 
+  //   decreases ss
+  // {
+  //   if ss == [] then {} else ss[0].FVars() + SeqFVars(ss[1..])
+  // }
+
+  // function SeqBVars(ss: seq<Stmt>): set<Variable> {
+  //   if ss == [] then {} else ss[0].BVars() + SeqBVars(ss[1..])
+  // }
 
   function Conj(ctx: seq<Expr>): Expr 
   {
     if ctx == [] then BConst(true) else And(ctx[0], Conj(ctx[1..]))
   }
 
-  lemma ConjFVarsMonotonicity(ctx1: seq<Expr>, ctx2: seq<Expr>)
+  lemma ConjDepthMonotonicity(ctx1: seq<Expr>, ctx2: seq<Expr>)
     requires ctx1 <= ctx2
-    ensures Conj(ctx1).FVars() <= Conj(ctx2).FVars()
+    ensures Conj(ctx1).Depth() <= Conj(ctx2).Depth()
   {  }
 
-  lemma FVarsConjUnionLemma(ctx1: seq<Expr>, ctx2: seq<Expr>)
-    ensures Conj(ctx1 + ctx2).FVars() == Conj(ctx1).FVars() + Conj(ctx2).FVars()
+  lemma DepthConjUnionLemma(ctx1: seq<Expr>, ctx2: seq<Expr>)
+    ensures Conj(ctx1 + ctx2).Depth() == max(Conj(ctx1).Depth(), Conj(ctx2).Depth())
   {
     if ctx1 == [] {
       assert [] + ctx2 == ctx2;
@@ -261,58 +312,62 @@ module Defs {
     }
   }
 
-  predicate SeqIsDefinedOn(ss: seq<Stmt>, s: set<Variable>) 
-    ensures SeqIsDefinedOn(ss, s) <==> SeqFVars(ss) <= s
+  predicate SeqIsDefinedOn(ss: seq<Stmt>, d: nat) 
+    ensures SeqIsDefinedOn(ss, d) <==> SeqDepth(ss) <= d
   {
-    if ss == [] then true else ss[0].IsDefinedOn(s) && SeqIsDefinedOn(ss[1..], s)
+    if ss == [] then true else ss[0].IsDefinedOn(d) && SeqIsDefinedOn(ss[1..], d)
   }
 
   lemma IsDefinedOnAndLemma(e0: Expr, e1: Expr, s: State)
-    requires e0.IsDefinedOn(s.Keys) && e1.IsDefinedOn(s.Keys)
-    ensures And(e0, e1).IsDefinedOn(s.Keys) { }
-
-  lemma IsDefinedOnConjLemma(ctx: seq<Expr>, s: State)
-    requires forall e <- ctx :: e.IsDefinedOn(s.Keys)
-    ensures Conj(ctx).IsDefinedOn(s.Keys)
-    {
-      if ctx != [] { IsDefinedOnAndLemma(ctx[0], Conj(ctx[1..]), s); }
-    }
-
-  lemma EvalConjLemma(ctx: seq<Expr>, s: State)
-    requires forall e <- ctx :: e.IsDefinedOn(s.Keys)
-    requires forall e <- ctx :: s.Eval(e)
-    ensures (IsDefinedOnConjLemma(ctx, s); s.Eval(Conj(ctx)))
+    requires e0.IsDefinedOn(|s|) 
+    requires e1.IsDefinedOn(|s|)
+    ensures And(e0, e1).IsDefinedOn(|s|) 
   {  }
 
-  predicate SeqNoShadowingNested(ss: seq<Stmt>, ghost parent: Stmt := Seq(ss)) 
-    requires forall s <- ss :: s < parent
-    decreases parent, |ss|
+  lemma IsDefinedOnConjLemma(ctx: seq<Expr>, s: State)
+    requires forall e <- ctx :: e.IsDefinedOn(|s|)
+    ensures Conj(ctx).IsDefinedOn(|s|)
   {
-    forall s <- ss :: s.NoShadowing()
+    if ctx != [] { 
+      IsDefinedOnAndLemma(ctx[0], Conj(ctx[1..]), s); 
+    } 
   }
 
-  predicate SeqNoShadowing(ss: seq<Stmt>, ghost parent: Stmt := Seq(ss)) 
-    requires forall s <- ss :: s < parent
-    decreases parent, |ss| + 1
-  {
-    && SeqNoShadowingNested(ss, parent)
-    && (forall i, j :: 0 <= i < j < |ss| ==> ss[i].BVars() !! ss[j].BVars())
-  }
+  lemma EvalConjLemma(ctx: seq<Expr>, s: State)
+    requires forall e <- ctx :: e.IsDefinedOn(|s|)
+    requires forall e <- ctx :: s.Eval(e)
+    ensures Conj(ctx).IsDefinedOn(|s|)
+    ensures s.Eval(Conj(ctx))
+  { IsDefinedOnConjLemma(ctx, s); }
 
-  predicate SeqWellFormed(ss: seq<Stmt>) {
-    if ss == [] then 
-      true 
-    else 
-      && ss[0].WellFormed()
-      && ss[0].BVars() !! SeqFVars(ss[1..]) 
-      && ss[0].BVars() !! SeqBVars(ss[1..])
-      && SeqWellFormed(ss[1..])
-  }
+  // predicate SeqNoShadowingNested(ss: seq<Stmt>, ghost parent: Stmt := Seq(ss)) 
+  //   requires forall s <- ss :: s < parent
+  //   decreases parent, |ss|
+  // {
+  //   forall s <- ss :: s.NoShadowing()
+  // }
+
+  // predicate SeqNoShadowing(ss: seq<Stmt>, ghost parent: Stmt := Seq(ss)) 
+  //   requires forall s <- ss :: s < parent
+  //   decreases parent, |ss| + 1
+  // {
+  //   && SeqNoShadowingNested(ss, parent)
+  //   && (forall i, j :: 0 <= i < j < |ss| ==> ss[i].BVars() !! ss[j].BVars())
+  // }
+
+  // predicate SeqWellFormed(ss: seq<Stmt>) {
+  //   if ss == [] then 
+  //     true 
+  //   else 
+  //     && ss[0].WellFormed()
+  //     && ss[0].BVars() !! SeqFVars(ss[1..]) 
+  //     && ss[0].BVars() !! SeqBVars(ss[1..])
+  //     && SeqWellFormed(ss[1..])
+  // }
 
   lemma SeqFunConcatLemmas(ss1: seq<Stmt>, ss2: seq<Stmt>)
     ensures SeqSize(ss1 + ss2) == SeqSize(ss1) + SeqSize(ss2)
-    ensures SeqBVars(ss1 + ss2) == SeqBVars(ss1) + SeqBVars(ss2)
-    ensures SeqFVars(ss1 + ss2) == SeqFVars(ss1) + SeqFVars(ss2)
+    ensures SeqDepth(ss1 + ss2) == max(SeqDepth(ss1), SeqDepth(ss2))
   {
     if ss1 == [] {
       assert ss1 + ss2 == ss2;
@@ -324,23 +379,23 @@ module Defs {
 
   type Value = bool
 
-  newtype State = map<Variable, Value> {
+  newtype State = seq<Value> {
     
     function Eval(e: Expr): Value 
-      requires e.IsDefinedOn(this.Keys)
+      requires e.IsDefinedOn(|this|)
       decreases e
     {
       match e
-      case BConst(bvalue) => bvalue
-      case And(e0, e1) => Eval(e0) && Eval(e1)
-      case Or(e0, e1) => Eval(e0) || Eval(e1)
-      case Not(e) => !Eval(e)
+      case BConst(bvalue)  => bvalue
+      case And(e0, e1)     => Eval(e0) && Eval(e1)
+      case Or(e0, e1)      => Eval(e0) || Eval(e1)
+      case Not(e)          => !Eval(e)
       case Implies(e0, e1) => Eval(e0) ==> Eval(e1)
-      case Forall(v, body) => forall x: bool :: Update(v, x).Eval(body)
-      case Var(v) => this[v]
+      case Forall(v, body) => forall x: bool :: Update(x).Eval(body)
+      case BVar(v)         => this[v]
     }
-    function Update(v: Variable, val: Value): State {
-      this[v := val]
+    function Update(val: Value): State {
+      [val] + this
     }
   }
 }
