src/Sound/Semantics/BigStep.dfy
@@ -1,4 +1,4 @@
-module BigStep {
+/*module BigStep {
   import opened Defs
 
   export 
@@ -141,4 +141,4 @@ module BigStep {
       FrameLemma(ss[0], v, b, st, w);
     }
   }
-}
+}*/
